---
title: "Lambda Calculus (Long-form)"
date: 2022-10-25T04:28:13+01:00
draft: true
tags: [ "CS349", "Programming Languages", "Lambda Calculus", "Notes" ]
---
# Basic Lambda Calculus
Lambda calculus is a notation for representing *functions*, *variables*, function creation (*abstraction*), and *application*. What these words mean isn't important right now - let's focus first on the structure of Lambda Calculus, and then imbue it with meaning.

## Syntax
Our simplest component is the humble *variable*. We usually represent variables with lowercase letters, eg. $$x \in Variables $$

Next, we have *terms*, which we will denote by M, or some other capital letter. A variable can be a term, an abstraction can be a term, and an application can be a term.
$$M ::= x | \lambda x.M | (M M)$$
I recognise that this might not make a lot of sense right now: but remember, we're not trying to give meaning to any of this yet. We just want to be able to recognise the format of a valid *lambda expression*.

As implied above, an *abstraction* is anything taking the form $$\lambda x.M$$
Where x is some variable, and M is some term.

An *application* is just a sequence of terms written next to eachother, of the form $$(M M)$$

... and that's it. Again, this might not make much sense right now, but these few rules define the structure of any lambda expression. Think about the following few examples, and why they are valid lambda terms.

$$a$$
$$\lambda d.e$$
$$\lambda f. (\lambda g. f)$$
$$(j k)$$
$$\lambda p. (p (\lambda r. ((\lambda s. p) r)))$$

Try to apply the definition of a term backwards for each of them. For the 3rd one for example, we can see that it is of the form $$\lambda x.M$$ where $$x = f, M = (\lambda g. f)$$

Once you have a feel for that, think about why the following examples are **not** valid terms:
$$\lambda p$$
$$\lambda (d f). e$$
$$\lambda q. \lambda r.$$
$$\lambda \lambda a. (b a)$$

## Association
In LC, application associates to the left. What this actually means is that when we write out a sequence of terms without brackets
$$M N O P Q$$
We assume "implicit" brackets over the leftmost terms
$$(((M N) O) P) Q$$
This means we don't have to write as many brackets when we want to express this.

## Binding
By now, you're probably wondering what all the lambdas are about. 
A lambda *binds* the succeeding *variable* to a *scope*. The *scope* is the part of the term that comes after the dot.
Any variable which appears in a expression, but has not been bound, is a *free* variable.
The meaning of what a *free* or *bound* variable actually is will be explained soon, but for now it helps to be able to identify them in an expression.

$$\lambda x. y x$$
In this, x is a bound variable, but y is a free variable.

$$\lambda x. y z$$
y and z are both free variables. x is bound, but not used in the expression.

$$\lambda x. (\lambda y. y x) y$$
Here is where it is slightly more complex - x is bound by the first lambda, and y is bound by the second lambda. However, the final y is actually a *free* variable - the *scope* of the second lambda ends with the closed bracket. 

To avoid too many brackets, we can use some syntactic sugar to help make our (nested) abstractions more readable.
$$\lambda x. (\lambda y. M) \equiv \lambda x y. M$$
For example:
$$\lambda a. (\lambda b. (\lambda c. c b a)) \equiv \lambda a b c. c b a$$

## Substitution


# Introducing semantics
> Seize two meaningless constants from the void, and imbue them with meaning. [...] To birth an algebra into the world is a beautiful thing. - Kyle Kingsbury (aka Aphyr)

Now that we can write valid lambda expressions, we should understand what they mean.

Abstractions can be thought about like *functions*. They take some term(s) in, and spit some term out.
For example:
$$\lambda a. a$$
Is a very simple abstraction, which we can think about as taking a value and returning it. 
We use *application* on abstractions to "pass" them a value.
$$(\lambda a. a) b \rightarrow b$$
This intuitively makes sense - the value a gets *bound* to the variable a, and the *scope* of the abstraction gets returned, replacing bound variables by their values. Let's formalise this rule, with some new notation.


[Return to Index ‚ü∂](/posts/cs349-index/)